removed dependency on Classes.v

src/coq/Error.v
@@ -8,17 +8,25 @@
  *   3 of the License, or (at your option) any later version.                 *
  ---------------------------------------------------------------------------- *)
 
-Require Import Vellvm.Classes Vellvm.Util.
-Require Import Program Classical.
-Require Import paco.
-Require Import ITree.
+Require Import String.
+Require Import ExtLib.Structures.Monads.
+Require Export ExtLib.Data.Monads.EitherMonad.
 
-Set Implicit Arguments.
-Set Contextual Implicit.
+Definition err T := sum string T.
 
-
-Instance functor_M {E} : Functor (M E) := (@mapM E).
-Instance monad_M {E} : (@Monad (M E)) (@mapM E) := { mret X x := Ret x; mbind := @bindM E }.
+Instance Monad_err : Monad err := Monad_either string.
+Instance Exception_err : MonadExc string err := Exception_either string.
 
 
+Definition trywith {E A:Type} {F} `{Monad F} `{MonadExc E F} (e:E) (o:option A) : F A :=
+    match o with
+    | Some x => ret x
+    | None => raise e
+    end.
+Hint Unfold trywith.
+Arguments trywith _ _ _ _ _: simpl nomatch.
+
+Definition failwith {A:Type} {F} `{Monad F} `{MonadExc string F} (s:string) : F A := raise s.
+Hint Unfold failwith.
+Arguments failwith _ _ _ _: simpl nomatch.
 
