src/coq/DeadInstr.v
@@ -10,7 +10,7 @@
 
 Require Import ZArith List String Omega.
 Require Import Program.
-Require Import  Vellvm.Classes Vellvm.Util.
+Require Import Vellvm.Util.
 Require Import Vellvm.LLVMAst Vellvm.AstLib Vellvm.CFG Vellvm.CFGProp.
 Import ListNotations.
 Open Scope Z_scope.
