src/coq/DecidableProp.v
@@ -6,7 +6,6 @@ Require Import compcert.lib.Integers.
 
 (* Vellvm dependencies *)
 Require Import Vellvm.LLVMAst Vellvm.CFG Vellvm.StepSemantics Vellvm.Memory.
-Require Import Vellvm.Classes.
 Require Import Vellvm.AstLib.
 Require Import Vellvm.DecidableEquality.
 
