src/coq/DynamicValues.v
@@ -10,14 +10,25 @@
 
 Require Import ZArith List String Omega.
 Require Import compcert.lib.Integers compcert.lib.Floats.
-Require Import Vellvm.Classes.
+Require Import ExtLib.Core.RelDec.
+Require Import ExtLib.Programming.Eqv.
+Require Import ExtLib.Structures.Monads.
+Require Import ExtLib.Data.Nat.
 Require Import Vellvm.LLVMAst.
 Require Import Vellvm.MemoryAddress.
+Require Import Vellvm.Error.
+Require Import Vellvm.Util.
+
+Import EqvNotation.
+Import MonadNotation.
+Import ListNotations.
 
 Set Implicit Arguments.
 Set Contextual Implicit.
 
 Open Scope Z_scope.
+
+Instance Eqv_nat : Eqv nat := (@eq nat).
 
 (* Set up representations for for i1, i32, and i64 *)
 Module Wordsize1.
@@ -378,14 +389,15 @@ Class VInt I : Type :=
 
   (* Arithmetic Operations ---------------------------------------------------- *)
   Section ARITHMETIC.
-    
+
+
   (* Evaluate integer opererations to get a dvalue.
 
      These operations are between VInts, which are "vellvm"
      integers. This is a typeclass that wraps all of the integer
      operations that we use for integer types with different bitwidths.
    *)
-  Definition eval_int_op `{VInt Int} (iop:ibinop) (x y: Int) : dvalue:=
+  Definition eval_int_op {Int} `{VInt Int} (iop:ibinop) (x y: Int) : dvalue:=
     match iop with
     (* Following to cases are probably right since they use CompCert *)
     | Add nuw nsw =>
@@ -396,9 +408,10 @@ Class VInt I : Type :=
       if orb (andb nuw (eq (sub_borrow x y zero) one))
              (andb nsw (eq (sub_overflow x y zero) one))
       then DVALUE_Poison else to_dvalue (sub x y)
+
     | Mul nuw nsw =>
       (* I1 mul can't overflow, just based on the 4 possible multiplications. *)
-      if (bitwidth == 1)%nat then to_dvalue (mul x y)
+      if (bitwidth ~=? 1)%nat then to_dvalue (mul x y)
       else 
         let res := mul x y in
         let res_s' := (signed x) * (signed y) in
@@ -407,8 +420,9 @@ Class VInt I : Type :=
              (andb nsw (orb (min_signed >? res_s')
                             (res_s' >? max_signed)))
       then DVALUE_Poison else to_dvalue res
+  
     | Shl nuw nsw =>
-      if (bitwidth == 1)%nat
+      if (bitwidth ~=? 1)%nat
       then
         if (unsigned y) >=? 1 then undef_int else to_dvalue x
       else
@@ -433,7 +447,7 @@ Class VInt I : Type :=
       if andb ex (negb (((signed x) mod (signed y)) =? 0))
       then DVALUE_Poison else to_dvalue (divs x y)
     | LShr ex =>
-      if (bitwidth == 1)%nat
+      if (bitwidth ~=? 1)%nat
       then
         if (unsigned y) >=? 1 then undef_int else to_dvalue x
       else
@@ -443,7 +457,7 @@ Class VInt I : Type :=
                                  mod (Z.pow 2 (unsigned y)) =? 0))
              then DVALUE_Poison else to_dvalue (shru x y)
     | AShr ex =>
-      if (bitwidth == 1)%nat
+      if (bitwidth ~=? 1)%nat
       then
         if (unsigned y) >=? 1 then undef_int else to_dvalue x
       else
@@ -467,13 +481,15 @@ Class VInt I : Type :=
   Arguments eval_int_op _ _ _ : simpl nomatch.
 
 
+  
+
   (* Evaluate the given iop on the given arguments according to the bitsize *)
   Definition integer_op (bits:Z) (iop:ibinop) (x y:inttyp bits) : err dvalue :=
     match bits, x, y with
-    | 1, x, y => mret (eval_int_op iop x y)
-    | 8, x, y => mret (eval_int_op iop x y)
-    | 32, x, y => mret (eval_int_op iop x y)
-    | 64, x, y => mret (eval_int_op iop x y)
+    | 1, x, y => ret (eval_int_op iop x y)
+    | 8, x, y => ret (eval_int_op iop x y)
+    | 32, x, y => ret (eval_int_op iop x y)
+    | 64, x, y => ret (eval_int_op iop x y)
     | _, _, _ => failwith "unsupported bitsize"
     end.
   Arguments integer_op _ _ _ _ : simpl nomatch.
@@ -482,20 +498,20 @@ Class VInt I : Type :=
      Takes the integer modulo 2^bits. *)
   Definition coerce_integer_to_int (bits:Z) (i:Z) : err dvalue :=
     match bits with
-    | 1 => mret (DVALUE_I1 (repr i))
-    | 8 => mret (DVALUE_I8 (repr i))
-    | 32 => mret (DVALUE_I32 (repr i))
-    | 64 => mret (DVALUE_I64 (repr i))
+    | 1 => ret (DVALUE_I1 (repr i))
+    | 8 => ret (DVALUE_I8 (repr i))
+    | 32 => ret (DVALUE_I32 (repr i))
+    | 64 => ret (DVALUE_I64 (repr i))
     | _ => failwith "unsupported integer size"
     end.
   Arguments coerce_integer_to_int _ _ : simpl nomatch.
 
   (* Helper for looping 2 argument evaluation over vectors, producing a vector *)
-  Fixpoint vec_loop (f:dvalue -> dvalue -> err dvalue) (elts:list (dvalue * dvalue))
-    : err (list dvalue) :=
+
+  Fixpoint vec_loop (f:dvalue -> dvalue -> err dvalue) (elts:list (dvalue * dvalue)) : err (list dvalue) :=
     monad_fold_right (fun acc '(e1, e2) =>
-                         'val <- f e1 e2;
-                         mret (val :: acc)
+                         val <- f e1 e2 ;;
+                         ret (val :: acc)
                        ) elts [].
 
   (* Integer iop evaluation, called from eval_iop.
@@ -503,10 +519,10 @@ Class VInt I : Type :=
      in order to prevent eval_iop from being recursive. *)
   Definition eval_iop_integer_h iop v1 v2 : err dvalue :=
     match v1, v2 with
-    | DVALUE_I1 i1, DVALUE_I1 i2 => mret (eval_int_op iop i1 i2)
-    | DVALUE_I8 i1, DVALUE_I8 i2 => mret (eval_int_op iop i1 i2)
-    | DVALUE_I32 i1, DVALUE_I32 i2 => mret (eval_int_op iop i1 i2)
-    | DVALUE_I64 i1, DVALUE_I64 i2 => mret (eval_int_op iop i1 i2)
+    | DVALUE_I1 i1, DVALUE_I1 i2 => ret (eval_int_op iop i1 i2)
+    | DVALUE_I8 i1, DVALUE_I8 i2 => ret (eval_int_op iop i1 i2)
+    | DVALUE_I32 i1, DVALUE_I32 i2 => ret (eval_int_op iop i1 i2)
+    | DVALUE_I64 i1, DVALUE_I64 i2 => ret (eval_int_op iop i1 i2)
     | _, _ => failwith "ill_typed-iop"
     end.
   Arguments eval_iop_integer_h _ _ _ : simpl nomatch.
@@ -517,14 +533,14 @@ Class VInt I : Type :=
   Definition eval_iop iop v1 v2 : err dvalue :=
     match v1, v2 with
     | (DVALUE_Vector elts1), (DVALUE_Vector elts2) =>
-      'val <- vec_loop (eval_iop_integer_h iop) (List.combine elts1 elts2);
-      mret (DVALUE_Vector val)
+      val <- vec_loop (eval_iop_integer_h iop) (List.combine elts1 elts2) ;;
+      ret (DVALUE_Vector val)
     | _, _ => eval_iop_integer_h iop v1 v2
     end.
   Arguments eval_iop _ _ _ : simpl nomatch.
 
 
-  Definition eval_int_icmp `{VInt Int} icmp (x y : Int) : dvalue :=
+  Definition eval_int_icmp {Int} `{VInt Int} icmp (x y : Int) : dvalue :=
     if match icmp with
        | Eq => cmp Ceq x y
        | Ne => cmp Cne x y
@@ -542,10 +558,10 @@ Class VInt I : Type :=
 
   Definition eval_icmp icmp v1 v2 : err dvalue :=
     match v1, v2 with
-    | DVALUE_I1 i1, DVALUE_I1 i2 => mret (eval_int_icmp icmp i1 i2)
-    | DVALUE_I8 i1, DVALUE_I8 i2 => mret (eval_int_icmp icmp i1 i2)
-    | DVALUE_I32 i1, DVALUE_I32 i2 => mret (eval_int_icmp icmp i1 i2)
-    | DVALUE_I64 i1, DVALUE_I64 i2 => mret (eval_int_icmp icmp i1 i2)
+    | DVALUE_I1 i1, DVALUE_I1 i2 => ret (eval_int_icmp icmp i1 i2)
+    | DVALUE_I8 i1, DVALUE_I8 i2 => ret (eval_int_icmp icmp i1 i2)
+    | DVALUE_I32 i1, DVALUE_I32 i2 => ret (eval_int_icmp icmp i1 i2)
+    | DVALUE_I64 i1, DVALUE_I64 i2 => ret (eval_int_icmp icmp i1 i2)
     | _, _ => failwith "ill_typed-icmp"
     end.
   Arguments eval_icmp _ _ _ : simpl nomatch.
@@ -553,19 +569,19 @@ Class VInt I : Type :=
 
   Definition double_op (fop:fbinop) (v1:ll_double) (v2:ll_double) : err dvalue :=
     match fop with
-    | FAdd => mret (DVALUE_Double (Float.add v1 v2))
-    | FSub => mret (DVALUE_Double (Float.sub v1 v2))
-    | FMul => mret (DVALUE_Double (Float.mul v1 v2))
-    | FDiv => mret (DVALUE_Double (Float.div v1 v2))
+    | FAdd => ret (DVALUE_Double (Float.add v1 v2))
+    | FSub => ret (DVALUE_Double (Float.sub v1 v2))
+    | FMul => ret (DVALUE_Double (Float.mul v1 v2))
+    | FDiv => ret (DVALUE_Double (Float.div v1 v2))
     | FRem => failwith "unimplemented"
     end.
 
   Definition float_op (fop:fbinop) (v1:ll_float) (v2:ll_float) : err dvalue :=
     match fop with
-    | FAdd => mret (DVALUE_Float (Float32.add v1 v2))
-    | FSub => mret (DVALUE_Float (Float32.sub v1 v2))
-    | FMul => mret (DVALUE_Float (Float32.mul v1 v2))
-    | FDiv => mret (DVALUE_Float (Float32.div v1 v2))
+    | FAdd => ret (DVALUE_Float (Float32.add v1 v2))
+    | FSub => ret (DVALUE_Float (Float32.sub v1 v2))
+    | FMul => ret (DVALUE_Float (Float32.mul v1 v2))
+    | FDiv => ret (DVALUE_Float (Float32.div v1 v2))
     | FRem => failwith "unimplemented"
     end.
 
@@ -634,8 +650,8 @@ Class VInt I : Type :=
 
   Definition eval_fcmp (fcmp:fcmp) (v1:dvalue) (v2:dvalue) : err dvalue :=
     match v1, v2 with
-    | DVALUE_Float f1, DVALUE_Float f2 => mret (float_cmp fcmp f1 f2)
-    | DVALUE_Double f1, DVALUE_Double f2 => mret (double_cmp fcmp f1 f2)
+    | DVALUE_Float f1, DVALUE_Float f2 => ret (float_cmp fcmp f1 f2)
+    | DVALUE_Double f1, DVALUE_Double f2 => ret (double_cmp fcmp f1 f2)
     | _, _ => failwith "ill_typed-fcmp"
     end.
 
@@ -646,7 +662,7 @@ Class VInt I : Type :=
   Definition eval_select_h cnd v1 v2 : err dvalue :=
     match cnd with
     | DVALUE_I1 i =>
-      mret (if Int1.unsigned i =? 1 then v1 else v2)
+      ret (if Int1.unsigned i =? 1 then v1 else v2)
     | _ => failwith "ill_typed-select"
     end.
   Arguments eval_select_h _ _ _ : simpl nomatch.
@@ -659,14 +675,14 @@ Class VInt I : Type :=
          generalize vec_loop to cover this? (make v1,v2 generic?) *)
       let fix loop elts :=
           match elts with
-          | [] => mret []
+          | [] => ret []
           | (cnd,(v1,v2)) :: tl =>
-              'val <- eval_select_h cnd v1 v2;
-              'vec <- loop tl;
-              mret (val :: vec)
+              val <- eval_select_h cnd v1 v2 ;;
+              vec <- loop tl ;;
+              ret (val :: vec)
           end in
-      'val <- loop (List.combine es (List.combine es1 es2));
-      mret (DVALUE_Vector val)
+      val <- loop (List.combine es (List.combine es1 es2)) ;;
+      ret (DVALUE_Vector val)
     | _, _, _ => eval_select_h cnd v1 v2
     end.
   Arguments eval_select _ _ _ : simpl nomatch.
@@ -678,7 +694,7 @@ Class VInt I : Type :=
         match elts with
         | [] => failwith "index out of bounds"
         | h :: tl =>
-          if idx =? 0 then mret h else loop tl (i-1)
+          if idx =? 0 then ret h else loop tl (i-1)
         end in
     match v with
     | DVALUE_Struct f => loop f idx
@@ -693,17 +709,17 @@ Class VInt I : Type :=
         match elts with
         | [] => failwith "index out of bounds"
         | h :: tl =>
-          if idx =? 0 then mret (acc ++ (v :: tl))
+          if idx =? 0 then ret (acc ++ (v :: tl))
           else loop (acc ++ [h]) tl (i-1)
         end%list in
     match str with
     | DVALUE_Struct f =>
-      'v <- (loop [] f idx);
-      mret (DVALUE_Struct v)
+      v <- (loop [] f idx) ;;
+      ret (DVALUE_Struct v)
 
     | DVALUE_Array e =>
-      'v <- (loop [] e idx);
-      mret (DVALUE_Array v)
+      v <- (loop [] e idx) ;;
+      ret (DVALUE_Array v)
 
     | _ => failwith "invalid aggregate data"
     end.
