src/coq/MMIO.v
@@ -1,4 +1,4 @@
 Require Import ZArith List String Omega.
-Require Import Vellvm.Classes Vellvm.Util Vellvm.Trace.
+Require Import Vellvm.Util Vellvm.Trace.
 
 
