src/coq/TypeUtil.v
@@ -3,7 +3,6 @@ Require Import Vellvm.Util.
 Require Import Vellvm.LLVMAst.
 Require Import Vellvm.AstLib.
 Require Import Vellvm.LLVMIO.
-Require Import Vellvm.Classes.
 Require Import Coqlib.
 Require Import Coq.Logic.FunctionalExtensionality.
 
